improved typing of bound variables; added support for user-provided Lemmas encoded to the solver; format.fst goes through

src/absyn/const.fs
@@ -139,6 +139,8 @@ let all_bind_lid    = p2l ["Prims";"ALL";"bind"]
 let ml_effect_lid   = p2l ["Prims"; "ALL"; "ML"]
 let assert_pure_lid = p2l ["Prims"; "PURE"; "assert_p"]
 let assume_pure_lid = p2l ["Prims"; "PURE"; "assume_p"]
+let fact_lid        = pconst "Fact"
+let lemma_lid       = pconst "Lemma"
 
 (* relational mode constants *)
 let lproj_lid            = pconst  "L"
