src/basic/util.fsi
@@ -98,6 +98,7 @@ val read_JSON: string -> 'a
 val int_of_string: string -> int
 val int_of_char:   char -> Tot<int>
 val char_of_int:   int -> Tot<char>
+val int_of_uint8: uint8 -> Tot<int>
 val uint16_of_int: int -> Tot<uint16>
 val float_of_byte: byte -> Tot<float>
 val float_of_int32: int32 -> Tot<float>
