examples/unit-tests/format.fst
@@ -1,64 +1,97 @@
+(*
+   Copyright 2008-2014 Nikhil Swamy and Microsoft Research
+
+   Licensed under the Apache License, Version 2.0 (the "License");
+   you may not use this file except in compliance with the License.
+   You may obtain a copy of the License at
+
+       http://www.apache.org/licenses/LICENSE-2.0
+
+   Unless required by applicable law or agreed to in writing, software
+   distributed under the License is distributed on an "AS IS" BASIS,
+   WITHOUT WARRANTIES OR CONDITIONS OF ANY KIND, either express or implied.
+   See the License for the specific language governing permissions and
+   limitations under the License.
+*)
+
 module Format
 open Prims.PURE
 open String
 open Array
 
-
-type message = seq char
+type message = seq byte
 type msg (l:nat) = m:message{length m==l}
 
-val append_inj_l: l:nat
+(* Here's a small proof that append is injective. 
+   To use this property, you have to explicitly call append_inj yourself (with an implicit first arg) *)
+val append_inj: #l:nat
+               -> b1:msg l -> b2:message
+               -> c1:msg l -> c2:message{append b1 b2==append c1 c2}
+               -> Fact unit
+                      (ensures (Equal b1 c1 /\ Equal b2 c2))
+let rec append_inj l b1 b2 c1 c2 = match l with
+  | 0 -> ()
+  | _ -> append_inj #(l - 1) (slice b1 1 l) b2 (slice c1 1 l) c2
+
+
+(* The same proof again, 
+   But, if you give it a "Lemma" type the solver 
+   will use the lemma as needed to prove other goals. *)
+val append_inj_lemma: l:nat (* NS: should eventually be able to drop this argument, once we have a syntax for decreases clause; for now, we need it to prove termination. *)
                -> b1:message -> b2:message
                -> c1:message -> c2:message
-               -> Pure unit
-                       (requires (l==length b1 /\ l==length c1 /\ append b1 b2==append c1 c2))
-                       (ensures \x -> (Equal b1 c1 /\ Equal b2 c2))
-let rec append_inj_l l b1 b2 c1 c2 = match l with
+               -> Lemma (requires (length b1==l /\ length b1==length c1 /\ append b1 b2==append c1 c2))
+                        (ensures (Equal b1 c1 /\ Equal b2 c2))
+                        [] (* VPat (append b1 b2); VPat (append c1 c2)] once we remove l:nat, adding these patterns will improve solver performance *)
+let rec append_inj_lemma l b1 b2 c1 c2 (* {decreases (length b1)} *) = 
+  match length b1 with
   | 0 -> ()
-  | _ -> append_inj_l (l - 1) (slice b1 1 l) b2 (slice c1 1 l) c2
+  | _ -> append_inj_lemma (l - 1) (slice b1 1 l) b2 (slice c1 1 l) c2
 
+let tag0 = create 1 0uy
+let tag1 = create 1 1uy
 
-(* let tag0 = create 1 0uy *)
-(* let tag1 = create 1 1uy *)
+logic type UInt16 (i:int) = (0 <= i /\ i < 65536)
+type uint16 = i:int{UInt16 i}
 
-(* type UInt16 (i:int) = (b2t (0 <= i) /\ b2t (i < 65536)) *)
-(* type uint16 = i:int{UInt16 i} *)
-(* assume logic val utf8: s:string -> Tot (m:message{length m <= strlen s}) //this spec is accurate for ASCII strings *)
-(* assume logic val two:nat *)
-(* assume logic val uint16_to_bytes: uint16 -> Tot (msg two) *)
-(* type string16 = s:string{UInt16 (length (utf8 s))} *)
+assume val utf8: s:string -> Tot (m:message{length m <= strlen s}) (* this spec is accurate for ASCII strings *)
+assume UTF8_inj: forall s0 s1.{:pattern (utf8 s0); (utf8 s1)}  Equal (utf8 s0) (utf8 s1) ==> s0==s1
 
-(* (\* assume UTF8_inj:   forall s0 s1.{:pattern (Equal (utf8 s0) (utf8 s1))} utf8 s0==utf8 s1 ==> s0==s1 *\) *)
-(* assume UINT16_inj: forall s0 s1. Equal (uint16_to_bytes s0) (uint16_to_bytes s1) *)
-(*                              ==> s0==s1 *)
+assume val uint16_to_bytes: uint16 -> Tot (msg 2)
+assume UINT16_inj: forall s0 s1. Equal (uint16_to_bytes s0) (uint16_to_bytes s1)
+                             ==> s0==s1
 
-(* logic val request : string -> Tot message *)
-(* let request s = append tag0 (utf8 s) *)
+type string16 = s:string{UInt16 (length (utf8 s))}
 
-(* logic val response: string16 -> string -> Tot message *)
-(* let response s t = *)
-(*   let lb = uint16_to_bytes (length (utf8 s)) in *)
-(*   append tag1 (append lb  *)
-(*                       (append (utf8 s)  *)
-(*                               (utf8 t))) *)
+val request : string -> Tot message
+let request s = append tag0 (utf8 s)
 
-(* (\* ask !v,v',s,s',t'. (Requested(v,s) /\ Responded(v',s',t')) -> (v <> v') *\) *)
-(* (\* lemma *\)  *)
-(* val req_resp_distinct: s:string -> s':string16 -> t':string -> Tot (u:unit{request s =!= response s' t'}) *)
-(* let req_resp_distinct s s' t' = () *)
+val response: string16 -> string -> Tot message
+let response s t =
+  let lb = uint16_to_bytes (length (utf8 s)) in
+  append tag1 (append lb
+                      (append (utf8 s)
+                              (utf8 t)))
 
-(* query ReqInj: forall s s'. request s==request s' ==> s==s' *)
+val req_resp_distinct: s:string -> s':string16 -> t':string
+                     -> Fact unit (ensures (~(Equal (request s) (response s' t'))))
+let req_resp_distinct s s' t' = ()
 
-(* (\* ask !v,s,s',t,t'. (Responded(v,s,t) /\ Responded(v,s',t')) -> (s = s' /\ t = t') *\) *)
-(* (\* ask !v,v',s,s'. (Requested(v,s) /\ Requested(v',s') /\ v = v') -> (s = s') *\) *)
-(* (\* ask !v,s,s',t,t'. (Responded(v,s,t) /\ Responded(v,s',t')) -> (s = s' /\ t = t') *\) *)
-     
-     
+val req_inj: s1:string -> s2:string{request s1=request s2} -> Fact unit (ensures (s1==s2))
+let req_inj s1 s2 = ()
 
+val resp_components_corr: s1:string16 
+                       -> t1:string 
+                       -> s2:string16
+                       -> t2:string
+                       -> Lemma (requires (response s1 t1 == response s2 t2))
+                                (ensures  (s1==s2 /\ t1==t2))
+                                [VPat (response s1 t1); VPat (response s2 t2)]
+let resp_components_corr s1 t1 s2 t2 = ()
 
-                                                               
-                                                               
-
-
-
-
+val req_components_corr: s1:string
+                      -> s2:string
+                      -> Lemma (requires (request s1 == request s2))
+                               (ensures  (s1==s2))
+                               [VPat (request s1); VPat (request s2)]
+let req_components_corr s1 s2 = ()
